Refactor laws of sharing proofs and corresponding infrastructure, #71

Coq/src/Classes.v
@@ -7,8 +7,10 @@ Class Shareable (A : Type) :=
 
 Class Normalform (A B : Type) :=
   {
-    nf : Prog A -> Prog B;
+    nf  : Prog A -> Prog B;
+    nf' : A -> Prog B;
     nf_impure: forall s (pf : _ -> Prog A),
-        nf (impure (ext s pf)) = impure (ext s (fun p => nf (pf p)))
-
+        nf (impure (ext s pf)) = impure (ext s (fun p => nf (pf p)));
+    nf_pure : forall (x : A),
+        nf (pure x) = nf' x             
   }.
